cfrontend/Cshmgenproof.v
@@ -1890,7 +1890,7 @@ Proof.
   econstructor; eauto. constructor.
 
 - (* internal function *)
-  inv H. inv TR. monadInv H7.
+  inv H. inv TR. monadInv H6.
   exploit match_cont_is_call_cont; eauto. intros [A B].
   exploit match_env_alloc_variables; eauto.
   apply match_env_empty.
